theories/Pattern.v
@@ -13,15 +13,12 @@ Inductive strict : Set :=
   | App (curried : strict) (argument : Name.name)
   .
 
-
-
 Fixpoint strict_eq a b :=
   match a, b with
   | Ctr a, Ctr b => Constructor.eq a b
   | App ca aa, App cb ab => andb (strict_eq ca cb) (Name.eqb aa ab)
   | _, _ => false
   end.
-Arguments strict_eq a b.
 
 Lemma strict_eq_spec a b
   : Reflect.Bool (a = b) (strict_eq a b).
@@ -37,17 +34,39 @@ Qed.
 
 
 
-Variant pattern : Set :=
-  | Nam (name : Name.name)
-  | Pat (strict : strict)
+Variant move_or_reference : Set :=
+  | Mov (strict : strict)
+  | Ref (strict : strict)
   .
 
+Definition move_or_reference_eq a b :=
+  match a, b with
+  | Mov a, Mov b => strict_eq a b
+  | Ref a, Ref b => strict_eq a b
+  | _, _ => false
+  end.
 
+Lemma move_or_reference_eq_spec a b
+  : Reflect.Bool (a = b) (move_or_reference_eq a b).
+Proof.
+  destruct a; destruct b; cbn.
+  - destruct (strict_eq_spec strict0 strict1); constructor. { subst. reflexivity. } intro E. apply N. invert E. reflexivity.
+  - constructor. intro D. discriminate D.
+  - constructor. intro D. discriminate D.
+  - destruct (strict_eq_spec strict0 strict1); constructor. { subst. reflexivity. } intro E. apply N. invert E. reflexivity.
+Qed.
+
+
+
+Variant pattern : Set :=
+  | Nam (name : Name.name)
+  | Pat (move_or_reference : move_or_reference)
+  .
 
 Definition eq a b :=
   match a, b with
   | Nam a, Nam b => Name.eqb a b
-  | Pat a, Pat b => strict_eq a b
+  | Pat a, Pat b => move_or_reference_eq a b
   | _, _ => false
   end.
 
@@ -58,5 +77,6 @@ Proof.
   - destruct (Name.spec name name0); constructor. { subst. reflexivity. } intro E. apply N. invert E. reflexivity.
   - constructor. intro D. discriminate D.
   - constructor. intro D. discriminate D.
-  - destruct (strict_eq_spec strict0 strict1); constructor. { subst. reflexivity. } intro E. apply N. invert E. reflexivity.
+  - unfold eq. destruct (move_or_reference_eq_spec move_or_reference0 move_or_reference1); constructor. { subst. reflexivity. }
+    intro E. apply N. invert E. reflexivity.
 Qed.
