theories/Extract.v
@@ -1,5 +1,5 @@
 From LinearCore Require
-  Map
+  Match
   .
 
 Set Extraction Optimize.
